mark-and-sweep/snapshot/internal/GC_Spec_GC_Lib_Header_GC_Lib_Address.h
@@ -10,6 +10,8 @@
 
 #include "krmllib.h"
 
+extern uint64_t GC_Spec_Base_heap_size_u64;
+
 #define GC_Lib_Header_White 0
 #define GC_Lib_Header_Gray 1
 #define GC_Lib_Header_Blue 2
@@ -18,8 +20,6 @@
 typedef uint8_t GC_Lib_Header_color_sem;
 
 bool GC_Lib_Header_uu___is_Black(GC_Lib_Header_color_sem projectee);
-
-extern uint64_t GC_Spec_Base_heap_size_u64;
 
 
 #define internal_GC_Spec_GC_Lib_Header_GC_Lib_Address_H_DEFINED
